gmap_view_auth: add fraction

theories/algebra/lib/gmap_view.v
@@ -132,8 +132,8 @@ Definition gmap_viewO (K : Type) `{Countable K} (V : ofeT) : ofeT :=
 Section definitions.
   Context {K : Type} `{Countable K} {V : ofeT}.
 
-  Definition gmap_view_auth (m : gmap K V) : gmap_viewR K V :=
-    ●V m.
+  Definition gmap_view_auth (q : frac) (m : gmap K V) : gmap_viewR K V :=
+    ●V{q} m.
   Definition gmap_view_frag (k : K) (dq : dfrac) (v : V) : gmap_viewR K V :=
     ◯V {[k := (dq, to_agree v)]}.
 End definitions.
@@ -142,10 +142,10 @@ Section lemmas.
   Context {K : Type} `{Countable K} {V : ofeT}.
   Implicit Types (m : gmap K V) (k : K) (q : Qp) (dq : dfrac) (v : V).
 
-  Global Instance : Params (@gmap_view_auth) 4 := {}.
-  Global Instance gmap_view_auth_ne : NonExpansive (gmap_view_auth (K:=K) (V:=V)).
+  Global Instance : Params (@gmap_view_auth) 5 := {}.
+  Global Instance gmap_view_auth_ne q : NonExpansive (gmap_view_auth (K:=K) (V:=V) q).
   Proof. solve_proper. Qed.
-  Global Instance gmap_view_auth_proper : Proper ((≡) ==> (≡)) (gmap_view_auth (K:=K) (V:=V)).
+  Global Instance gmap_view_auth_proper q : Proper ((≡) ==> (≡)) (gmap_view_auth (K:=K) (V:=V) q).
   Proof. apply ne_proper, _. Qed.
 
   Global Instance : Params (@gmap_view_frag) 6 := {}.
@@ -171,10 +171,30 @@ Section lemmas.
   Qed.
 
   (** Composition and validity *)
-  Lemma gmap_view_auth_valid m : ✓ gmap_view_auth m.
+  Lemma gmap_view_auth_frac_valid m q : ✓ gmap_view_auth q m ↔ ✓ q.
   Proof.
-    apply view_auth_valid. intros n l ? Hl. rewrite lookup_empty in Hl. done.
+    rewrite view_auth_frac_valid. split; first by naive_solver.
+    intros. split; first done.
+    intros n l ? Hl. rewrite lookup_empty in Hl. done.
   Qed.
+  Lemma gmap_view_auth_valid m : ✓ gmap_view_auth 1 m.
+  Proof. rewrite gmap_view_auth_frac_valid. done. Qed.
+
+  Lemma auth_auth_frac_op p q m :
+    gmap_view_auth (p + q) m ≡ gmap_view_auth p m ⋅ gmap_view_auth q m.
+  Proof. apply view_auth_frac_op. Qed.
+  Lemma auth_auth_frac_op_invN n p m1 q m2 :
+    ✓{n} (gmap_view_auth p m1 ⋅ gmap_view_auth q m2) → m1 ≡{n}≡ m2.
+  Proof. apply view_auth_frac_op_invN. Qed.
+  Lemma auth_auth_frac_op_inv p m1 q m2 :
+    ✓ (gmap_view_auth p m1 ⋅ gmap_view_auth q m2) → m1 ≡ m2.
+  Proof. apply view_auth_frac_op_inv. Qed.
+  Lemma auth_auth_frac_op_inv_L `{!LeibnizEquiv V} q m1 p m2 :
+    ✓ (gmap_view_auth p m1 ⋅ gmap_view_auth q m2) → m1 = m2.
+  Proof. apply view_auth_frac_op_inv_L, _. Qed.
+  Global Instance auth_auth_frac_is_op q q1 q2 m :
+    IsOp q q1 q2 → IsOp' (gmap_view_auth q m) (gmap_view_auth q1 m) (gmap_view_auth q2 m).
+  Proof. rewrite /gmap_view_auth. apply _. Qed.
 
   Lemma gmap_view_frag_validN n k dq v : ✓{n} gmap_view_frag k dq v ↔ ✓ dq.
   Proof.
@@ -213,28 +233,38 @@ Section lemmas.
     ✓ (gmap_view_frag k dq1 v1 ⋅ gmap_view_frag k dq2 v2) ↔ ✓ (dq1 ⋅ dq2) ∧ v1 = v2.
   Proof. unfold_leibniz. apply gmap_view_frag_op_valid. Qed.
 
-  Lemma gmap_view_both_validN n m k dq v :
-    ✓{n} (gmap_view_auth m ⋅ gmap_view_frag k dq v) ↔
-      ✓ dq ∧ m !! k ≡{n}≡ Some v.
+  Lemma gmap_view_both_frac_validN n q m k dq v :
+    ✓{n} (gmap_view_auth q m ⋅ gmap_view_frag k dq v) ↔
+      ✓ q ∧ ✓ dq ∧ m !! k ≡{n}≡ Some v.
   Proof.
     rewrite /gmap_view_auth /gmap_view_frag.
-    rewrite view_both_validN.
-    apply gmap_view_rel_lookup.
+    rewrite view_both_frac_validN gmap_view_rel_lookup.
+    naive_solver.
+  Qed.
+  Lemma gmap_view_both_validN n m k dq v :
+    ✓{n} (gmap_view_auth 1 m ⋅ gmap_view_frag k dq v) ↔
+      ✓ dq ∧ m !! k ≡{n}≡ Some v.
+  Proof. rewrite gmap_view_both_frac_validN. naive_solver done. Qed.
+  Lemma gmap_view_both_frac_valid q m k dq v :
+    ✓ (gmap_view_auth q m ⋅ gmap_view_frag k dq v) ↔
+    ✓ q ∧ ✓ dq ∧ m !! k ≡ Some v.
+  Proof.
+    rewrite /gmap_view_auth /gmap_view_frag.
+    rewrite view_both_frac_valid. setoid_rewrite gmap_view_rel_lookup.
+    split=>[[Hq Hm]|[Hq Hm]].
+    - split; first done. split.
+      +  apply (Hm 0%nat).
+      +  apply equiv_dist=>n. apply Hm.
+    - split; first done. split.
+      + apply Hm.
+      + revert n. apply equiv_dist. apply Hm.
   Qed.
   Lemma gmap_view_both_valid m k dq v :
-    ✓ (gmap_view_auth m ⋅ gmap_view_frag k dq v) ↔
+    ✓ (gmap_view_auth 1 m ⋅ gmap_view_frag k dq v) ↔
     ✓ dq ∧ m !! k ≡ Some v.
-  Proof.
-    rewrite /gmap_view_auth /gmap_view_frag.
-    rewrite view_both_valid. setoid_rewrite gmap_view_rel_lookup.
-    split; intros Hm; split.
-    - apply (Hm 0%nat).
-    - apply equiv_dist=>n. apply Hm.
-    - apply Hm.
-    - revert n. apply equiv_dist. apply Hm.
-  Qed.
+  Proof. rewrite gmap_view_both_frac_valid. naive_solver done. Qed.
   Lemma gmap_view_both_valid_L `{!LeibnizEquiv V} m k dq v :
-    ✓ (gmap_view_auth m ⋅ gmap_view_frag k dq v) ↔
+    ✓ (gmap_view_auth 1 m ⋅ gmap_view_frag k dq v) ↔
     ✓ dq ∧ m !! k = Some v.
   Proof. unfold_leibniz. apply gmap_view_both_valid. Qed.
 
@@ -242,7 +272,7 @@ Section lemmas.
   Lemma gmap_view_alloc m k dq v :
     m !! k = None →
     ✓ dq →
-    gmap_view_auth m ~~> gmap_view_auth (<[k := v]> m) ⋅ gmap_view_frag k dq v.
+    gmap_view_auth 1 m ~~> gmap_view_auth 1 (<[k := v]> m) ⋅ gmap_view_frag k dq v.
   Proof.
     intros Hfresh Hdq. apply view_update_alloc=>n bf Hrel j [df va] /=.
     rewrite lookup_op. destruct (decide (j = k)) as [->|Hne].
@@ -261,8 +291,8 @@ Section lemmas.
   Qed.
 
   Lemma gmap_view_delete m k v :
-    gmap_view_auth m ⋅ gmap_view_frag k (DfracOwn 1) v ~~>
-    gmap_view_auth (delete k m).
+    gmap_view_auth 1 m ⋅ gmap_view_frag k (DfracOwn 1) v ~~>
+    gmap_view_auth 1 (delete k m).
   Proof.
     apply view_update_dealloc=>n bf Hrel j [df va] Hbf /=.
     destruct (decide (j = k)) as [->|Hne].
@@ -276,8 +306,8 @@ Section lemmas.
   Qed.
 
   Lemma gmap_view_update m k v v' :
-    gmap_view_auth m ⋅ gmap_view_frag k (DfracOwn 1) v ~~>
-      gmap_view_auth (<[k := v']> m) ⋅ gmap_view_frag k (DfracOwn 1) v'.
+    gmap_view_auth 1 m ⋅ gmap_view_frag k (DfracOwn 1) v ~~>
+      gmap_view_auth 1 (<[k := v']> m) ⋅ gmap_view_frag k (DfracOwn 1) v'.
   Proof.
     apply view_update=>n bf Hrel j [df va] /=.
     rewrite lookup_op. destruct (decide (j = k)) as [->|Hne].
